Complexity/Lazy_Greedy_Compare_NaiveScan.thy
@@ -1,0 +1,157 @@
+theory Lazy_Greedy_Compare_NaiveScan
+  imports
+    Lazy_Greedy_TotalOracleCost
+    "../Core/Oracle_Cost"
+    "../Proofs/Lazy_Greedy_Stateful_StepSpec"
+begin
+
+context Cardinality_Constraint
+begin
+
+lemma step_gain_evals_le_card_remaining:
+  "step_gain_evals i \<le> card (remaining (lazy_state i))"
+proof -
+  let ?st = "lazy_state i"
+  let ?A  = "remaining ?st"
+  show ?thesis
+  proof (cases "?A = {}")
+    case True
+    then show ?thesis
+      by (simp add: step_gain_evals_def Let_def)
+  next
+    case False
+    have "step_gain_evals i = lazy_select_gain_evals (Sg ?st) ?A (ubg ?st)"
+      using False by (simp add: step_gain_evals_def Let_def)
+    also have "... \<le> card ?A"
+      using lazy_select_gain_evals_le_cardA by simp
+    finally show ?thesis by simp
+  qed
+qed
+
+lemma card_lazy_set_eq_index_upto:
+  assumes m_le: "m \<le> card V"
+  shows "\<And>i. i \<le> m \<Longrightarrow> card (lazy_set i) = i"
+proof -
+  fix i
+  assume i_le: "i \<le> m"
+  show "card (lazy_set i) = i"
+    using i_le
+  proof (induction i)
+    case 0
+    then show ?case
+      by (simp add: lazy_set_def init_state_def)
+  next
+    case (Suc i)
+    have i_le_m: "i \<le> m"
+      using Suc.prems by simp
+
+    have IH: "card (lazy_set i) = i"
+      using Suc.IH[OF i_le_m] .
+
+    have i_lt_m: "i < m"
+      using Suc.prems by simp
+
+    have i_lt_cardV: "i < card V"
+      using less_le_trans[OF i_lt_m m_le] .
+
+    have subV: "lazy_set i \<subseteq> V"
+      using lazy_state_subset_V[of i]
+      by (simp add: lazy_set_def)
+
+    have finS: "finite (lazy_set i)"
+      using finite_subset[OF subV finite_V] .
+
+    have rem_ne: "V - lazy_set i \<noteq> {}"
+    proof
+      assume empty: "V - lazy_set i = {}"
+      have V_sub: "V \<subseteq> lazy_set i"
+        using empty by auto
+      have eqV: "lazy_set i = V"
+        using subset_antisym[OF subV V_sub] by simp
+      have cardEq: "card (lazy_set i) = card V"
+        using eqV finite_V by simp
+      have i_eqV: "i = card V"
+        using IH cardEq by simp
+      show False
+        using i_eqV i_lt_cardV by simp
+    qed
+
+    have ins: "lazy_set (Suc i) = insert (lazy_choice i) (lazy_set i)"
+      using lazy_set_Suc_insert_V_minus_S[OF rem_ne] .
+
+    have xin: "lazy_choice i \<in> V - lazy_set i"
+      using lazy_choice_in_V_minus_S[OF rem_ne] .
+
+    have xnot: "lazy_choice i \<notin> lazy_set i"
+      using xin by simp
+
+    have cardSuc: "card (lazy_set (Suc i)) = Suc (card (lazy_set i))"
+      using ins finS xnot by simp
+
+    show ?case
+      using cardSuc IH by simp
+  qed
+qed
+
+(* C. Exact alignment with the standard scan baseline: remaining size = card V - i. *)
+lemma card_remaining_eq_cardV_minus_i:
+  assumes m_le: "m \<le> card V" and i_lt: "i < m"
+  shows "card (remaining (lazy_state i)) = card V - i"
+proof -
+  have subV: "lazy_set i \<subseteq> V"
+    using lazy_state_subset_V[of i] by (simp add: lazy_set_def)
+  have finS: "finite (lazy_set i)"
+    using finite_V subV by (meson finite_subset)
+  have cardS: "card (lazy_set i) = i"
+    using card_lazy_set_eq_index_upto[OF m_le] i_lt by simp
+
+  have "remaining (lazy_state i) = V - lazy_set i"
+    by (simp add: remaining_def lazy_set_def)
+
+  moreover have "card (V - lazy_set i) = card V - card (lazy_set i)"
+    using finite_V finS subV by (simp add: card_Diff_subset)
+
+  ultimately show ?thesis
+    using cardS by simp
+qed
+
+theorem total_gain_evals_le_naive_scan:
+  assumes m_le: "m \<le> card V"
+  shows "total_gain_evals m \<le> naive_greedy_gain_evals (card V) m"
+proof -
+  have step_le:
+    "\<And>i. i < m \<Longrightarrow> step_gain_evals i \<le> card V - i"
+  proof -
+    fix i assume i_lt: "i < m"
+    have "step_gain_evals i \<le> card (remaining (lazy_state i))"
+      by (rule step_gain_evals_le_card_remaining)
+    also have "... = card V - i"
+      using card_remaining_eq_cardV_minus_i[OF m_le i_lt] .
+    finally show "step_gain_evals i \<le> card V - i" .
+  qed
+
+  have tot_m: "total_gain_evals m \<le> (\<Sum>i<m. card V - i)"
+    by (rule tot_le[of m], simp)
+    by (induction m) (simp_all add: sum.lessThan_Suc)
+  also have "... = naive_greedy_gain_evals (card V) m"
+    by (simp add: naive_greedy_gain_evals_def)
+  finally show ?thesis .
+qed
+
+theorem total_oracle_calls_le_naive_scan:
+  assumes m_le: "m \<le> card V"
+  shows "total_oracle_calls m \<le> naive_greedy_oracle_calls (card V) m"
+proof -
+  have "gain_call_cost * total_gain_evals m \<le> gain_call_cost * naive_greedy_gain_evals (card V) m"
+    using total_gain_evals_le_naive_scan[OF m_le] by (simp add: mult_left_mono)
+  thus ?thesis
+    by (simp add: total_oracle_calls_def naive_greedy_oracle_calls_def)
+qed
+
+theorem total_oracle_calls_le_sum_untight:
+  "total_oracle_calls m \<le> gain_call_cost * (\<Sum>i<m. step_gain_bound_untight i)"
+  using total_gain_evals_le_sum_untight
+  by (simp add: total_oracle_calls_def mult_left_mono)
+
+end
+end
